link.v
@@ -17,9 +17,8 @@ Inductive dOp := memberOp | insertOp | deleteOp.
 Variable findNext : val.
 Variable decisiveOp : (dOp → val).
 Variable searchStrSpec : (dOp → val).
-Variable lockLoc : node → loc.
+Variable lockLoc : Node → loc.
 Variable getLockLoc : val.
-Variable ks: node → gset key.
 
 Definition lockNode : val :=
   rec: "lockN" "x" :=
@@ -41,7 +40,7 @@ Definition traverse : val :=
     | SOME "n'" => unlockNode "n";; "tr" "n'" "k"
     end.
 
-Definition searchStrOp (Ψ: dOp) (root: node) : val :=
+Definition searchStrOp (Ψ: dOp) (root: Node) : val :=
   rec: "dictOp" "k" :=
     let: "n" := traverse #root "k" in
     match: ((decisiveOp Ψ) "n" "k") with
@@ -59,8 +58,8 @@ Instance subG_flowintΣ {Σ} : subG flowintΣ Σ → flowintG Σ.
 Proof. solve_inG. Qed.
 
 (* RA for authoritative set of nodes *)
-Class nodesetG Σ := NodesetG { nodeset_inG :> inG Σ (authR (gsetUR node)) }.
-Definition nodesetΣ : gFunctors := #[GFunctor (authR (gsetUR node))].
+Class nodesetG Σ := NodesetG { nodeset_inG :> inG Σ (authR (gsetUR Node)) }.
+Definition nodesetΣ : gFunctors := #[GFunctor (authR (gsetUR Node))].
 
 Instance subG_nodesetΣ {Σ} : subG nodesetΣ Σ → nodesetG Σ.
 Proof. solve_inG. Qed.
@@ -92,63 +91,47 @@ Section Link_Template.
 
   (* ---------- Flow interface set-up specific to this proof ---------- *)
   
-  Parameter in_inset : key → flowintUR → node → Prop.
-  Parameter in_outset : key → flowintUR → node → Prop.
-  Parameter not_in_outset : key → flowintUR → Prop.
-  Parameter inreach : flowintUR → node → gset key.
+  Parameter in_inset : key → flowintUR → Node → Prop.
+  Parameter in_outset : key → flowintUR → Node → Prop.      
+  Parameter linkset : flowintUR → Node → gset key.               (*inreach → linkset*)
   Parameter is_empty_flowint : flowintUR → Prop.
+  Parameter keyset : flowintUR → Node → gset key.                 (* define as a lemma keyset I_n n *)
 
-  Variable root : node.    (* make root parameter of the specs *)
-  Variable KS : gset key.                                
-  Variable hrep : node → flowintUR → gset key → iProp.
-  Parameter hrep_timeless_proof : ∀ n I C, Timeless (hrep n I C).
-  Instance hrep_timeless n I C: Timeless (hrep n I C).
-  Proof. apply hrep_timeless_proof. Qed.
-  Parameter hrep_sep_star: ∀ n I_n I_n' C C', hrep n I_n C ∗ hrep n I_n' C' -∗ False.
-  Parameter KS_full : ∀ k, k ∈ KS.
+  Parameter node : Node → flowintUR → gset key → iProp.
+  Parameter node_timeless_proof : ∀ n I C, Timeless (node n I C).
+  Instance node_timeless n I C: Timeless (node n I C).
+  Proof. apply node_timeless_proof. Qed.
 
-  Definition globalint I : Prop := ✓I ∧ (∀ k n, ¬ (in_outset k I n)) ∧  (* For later, make outset and inset to be sets *)
-                                  (∀ n, (n = root) → (∀ k, in_inset k I n ∧ k ∈ inreach I n)
-                                      ∧ (n ≠ root) → (∀ k, ¬ in_inset k I n ∧ k ∉ inreach I n)).  
+  Definition in_outsets k In := ∃ n, in_outset k In n.
+
+  Definition globalint root I : Prop := ✓I ∧ (root ∈ dom I) ∧ (∀ k n, ¬ (in_outset k I n)) 
+                                  ∧ ∀ n, ((n = root) → (∀ k, in_inset k I n ∧ k ∈ linkset I n))
+                                      ∧ ((n ≠ root) → (∀ k, ¬ in_inset k I n ∧ k ∉ linkset I n)).
+
+  Definition nodeinv I_n n: Prop := (∀ k, k ∈ linkset I_n n ∧ ¬ in_outsets k I_n → in_inset k I_n n).    
 
   (* ---------- Proved in GRASShopper for each implementation: ---------- *)
 
-  (** follows from def of intComp - I suggest to fill in the definition of interface composition so that this one just follows from the definition in Coq as well. Otherwise, it should be moved to flows.v *)
-  Lemma flowint_comp_fp (I1 I2 I : flowintUR) : I = I1 ⋅ I2 → dom I = dom I1 ∪ dom I2.
-  Proof. Admitted.
+  Hypothesis keyset_def : ∀ k I_n n, in_inset k I_n n → ¬ in_outsets k I_n → k ∈ keyset I_n n.
 
-  (*done*)
-  Hypothesis globalint_root_fp: ∀ I, globalint I → root ∈ dom I.
-  (* part of nodeint *)
-  Hypothesis keyset_in_out : ∀ k In n, in_inset k In n → not_in_outset k In → k ∈ ks n.
+  Hypothesis node_sep_star: ∀ n I_n I_n' C C', node n I_n C ∗ node n I_n' C' -∗ False.
 
-  (* done *)
-  Hypothesis globalint_root_inr : ∀ I k, globalint I → k ∈ inreach I root. (* can be proved in coq itself *)
+  Hypothesis node_implies_nodeinv : ∀ n I_n C, (⌜✓I_n⌝)%I ∗ node n I_n C -∗ node n I_n C ∗ (⌜nodeinv I_n n⌝)%I. 
+                                                        (* check the name *)
+   
+  Hypothesis flowint_comp_fp : ∀ I1 I2 I, I = I1 ⋅ I2 → dom I = dom I1 ∪ dom I2.      (* move to the flows file *)
 
-  (* please rename to "inreach_monotone" and change it according to multipair-flows.spl *)
-  Hypothesis globalint_inreach :
-    ∀ Ir I, Ir ≼ I → dom Ir = {[root]} → globalint I → inreach Ir root = inreach I root.
-
-  (* done *)
+  Hypothesis inreach_monotone :                                           (* globalint_inreach → inreach_monotone *)
+    ∀ I I1 I2 k n,  ✓ I → I = I1⋅I2 → n ∈ dom I1 → k ∈ linkset I n → k ∈ linkset I1 n.
+      
   Hypothesis outset_distinct : ∀ I n, (∃ k, in_outset k I n) → n ∉ dom I. 
+  
+  Hypothesis flowint_inreach_step : 
+    ∀ I I1 I2 k n1 n2, ✓ I → I = I1⋅I2 → in_outset k I1 n2 → k ∈ linkset I1 n1 → k ∈ linkset I2 n2.
 
-  (* part of nodeint. Why does this need V(I)? *)
-  Lemma inreach_impl_inset I_n n k:
-    dom I_n = {[n]} → k ∈ inreach I_n n ∧ not_in_outset k I_n ∧ ✓ I_n → in_inset k I_n n.
-  Proof. Admitted.
-
-  (* todo *)
-  Lemma flowint_inreach_step (I I1 I2: flowintUR) k n n':
-    dom I1 = {[n]} → n' ∈ dom I2 → I = I1 ⋅ I2 → ✓(I)
-    → k ∈ inreach I1 n → in_outset k I1 n' → k ∈ inreach I2 n'.
-  Proof. Admitted.
-
-  (* done *)
-  Lemma flowint_step (I I1 I2: flowintUR) k n:
-    I = I1 ⋅ I2 → ✓I → in_outset k I1 n → globalint I → n ∈ dom I2.
-  Proof. Admitted.
-
-
+  Hypothesis flowint_step :
+    ∀ I I1 I2 k n root, I = I1 ⋅ I2 → ✓I → in_outset k I1 n → globalint root I → n ∈ dom I2.
+  
   (* ---------- Coarse-grained specification ---------- *)
 
   Definition Ψ dop k (C: gset key) (C': gset key) (res: bool) : iProp :=
@@ -164,44 +147,66 @@ Section Link_Template.
 
   (* ---------- Helper functions specs - proved for each implementation in GRASShopper ---------- *)
 
-  Parameter getLockLoc_spec : ∀ (n: node),
+  Parameter getLockLoc_spec : ∀ (n: Node),
       ({{{ True }}}
            getLockLoc #n
        {{{ (l:loc), RET #l; ⌜lockLoc n = l⌝ }}})%I.
 
-  Parameter findNext_spec : ∀ (n: node) (I_n : flowintUR) (C: gset key) (k: key),
-      ({{{ hrep n I_n C ∗ ⌜k ∈ inreach I_n n⌝ }}}
+  Parameter findNext_spec : ∀ (n: Node) (I_n : flowintUR) (C: gset key) (k: key),
+      ({{{ node n I_n C ∗ ⌜k ∈ linkset I_n n ∨ in_inset k I_n n⌝ }}}
            findNext #n #k
-       {{{ (b: bool) (n': node), 
+       {{{ (b: bool) (n': Node), 
               RET (match b with true => (SOMEV #n') | false => NONEV end); 
-               hrep n I_n C ∗ (match b with true => ⌜in_outset k I_n n'⌝ |
-                                          false => ⌜not_in_outset k I_n⌝ end) }}})%I.
+               node n I_n C ∗ (match b with true => ⌜in_outset k I_n n'⌝ |
+                                          false => ⌜¬in_outsets k I_n⌝ end) }}})%I.
 
-  Parameter decisiveOp_spec : ∀ (dop: dOp) (n: node) (k: key) (I_n: flowintUR) (C: gset key),
-      ({{{ hrep n I_n C ∗ ⌜in_inset k I_n n⌝
-                    ∗ ⌜not_in_outset k I_n⌝ }}}
+  Parameter decisiveOp_spec : ∀ (dop: dOp) (n: Node) (k: key) (I_n: flowintUR) (C: gset key),
+      ({{{ node n I_n C ∗ ⌜in_inset k I_n n⌝
+                    ∗ ⌜¬in_outsets k I_n⌝ }}}
            decisiveOp dop #n #k
        {{{ (b: bool) (C': gset key) (res: bool),
                   RET (match b with false => NONEV | true => (SOMEV #res) end);
-                  match b with false => hrep n I_n C |
-                              true => hrep n I_n C' ∗ Ψ dop k C C' res ∗ ⌜ C' ⊆ ks n⌝ end }}})%I.
+                  match b with false => node n I_n C |
+                              true => node n I_n C' ∗ Ψ dop k C C' res ∗ ⌜ C' ⊆ keyset I_n n⌝ end }}})%I.
 
   (* ---------- The invariant ---------- *)
   
 (* should change the name so as to not confuse with the node-level predicate *)
-  Definition searchStr γ γ_fp γ_k γ_inr γ_fi I C : iProp :=                             
-    (own γ (● I) ∗ own γ_k (● prod (KS, C)) ∗ own γ_fp (● dom I) ∗ ⌜globalint I⌝
-      ∗ ([∗ set] n ∈ (dom I), (∃ (b: bool) (In: flowintUR),
+  Definition searchStr γ γ_fp γ_k γ_inr γ_fi root I C : iProp :=                             
+    (own γ (● I) ∗ own γ_k (● prod (KS, C)) ∗ own γ_fp (● dom I) ∗ ⌜globalint root I⌝
+      ∗ ([∗ set] n ∈ (dom I), (∃ (b: bool) (I_n: flowintUR),
           (lockLoc n) ↦ #b
           ∗ (if b then True
-            else (∃ Cn, hrep n In Cn ∗ own (γ_fi n) ((●{1/2} In)) ∗ own γ_k (◯ prod (ks(n), Cn))))
-          ∗ own γ (◯ In) ∗ ⌜dom In = {[n]}⌝ ∗ own (γ_fi n) ((●{1/2} In)) ∗ own (γ_inr n) (● (inreach In n))
+            else (∃ C_n, node n I_n C_n ∗ own (γ_fi n) ((●{1/2} I_n)) ∗ own γ_k (◯ prod (keyset I_n n, C_n))))
+          ∗ own γ (◯ I_n) ∗ ⌜dom I_n = {[n]}⌝ ∗ own (γ_fi n) ((●{1/2} I_n)) ∗ own (γ_inr n) (● (linkset I_n n))
         ))
     )%I.    
 
-  Definition is_searchStr γ γ_fp γ_k γ_inr γ_fi C := (∃ I, (searchStr γ γ_fp γ_k γ_inr γ_fi I C))%I.
+  Definition is_searchStr γ γ_fp γ_k γ_inr γ_fi root C := (∃ I, (searchStr γ γ_fp γ_k γ_inr γ_fi root I C))%I.
 
   (* ---------- Assorted useful lemmas ---------- *)
+
+  Lemma globalint_root_fp: ∀ I root, globalint root I → root ∈ dom I.
+  Proof. 
+    intros I root Hglob. unfold globalint in Hglob.
+    destruct Hglob as [H1 [H2 H3]]. done.
+  Qed.    
+
+  Lemma globalint_root_inr : ∀ I Ir root k, globalint root I ∧ Ir ≼ I 
+                                           ∧ dom Ir = {[root]} → k ∈ linkset Ir root.
+  Proof.
+    intros I Ir root k Hglob. destruct Hglob as [Hglob [H1 H2]].
+    unfold globalint in Hglob. destruct Hglob as [H3 [H4 [H5 H6]]].
+    specialize (H6 root). assert (k ∈ linkset I root).
+    { apply H6. done. } destruct H1 as [I2 H1].
+     apply (inreach_monotone I Ir I2 k root); try done. set_solver.
+  Qed. 
+
+  Lemma auth_own_incl γ (x y: flowintUR) : own γ (● x) ∗ own γ (◯ y) -∗ ⌜y ≼ x⌝.
+  Proof.
+    rewrite -own_op. rewrite own_valid. iPureIntro.
+    apply auth_both_valid.
+  Qed.
 
   Lemma auth_set_incl γ_fp Ns Ns' :
     own γ_fp (◯ Ns) ∗ own γ_fp (● Ns') -∗ ⌜Ns ⊆ Ns'⌝.
@@ -211,13 +216,7 @@ Section Link_Template.
     intros. destruct H. inversion H0 as [m H1].
     destruct H1. destruct H2. apply gset_included in H2.
     apply to_agree_inj in H1. set_solver.
-  Qed.
-
-  Lemma auth_own_incl γ (x y: flowintUR) : own γ (● x) ∗ own γ (◯ y) -∗ ⌜y ≼ x⌝.
-  Proof.
-    rewrite -own_op. rewrite own_valid. iPureIntro.
-    apply auth_both_valid.
-  Qed.
+  Qed.  
 
   Lemma auth_own_incl_ks γ (x y: keysetUR) : own γ (● x) ∗ own γ (◯ y) -∗ ⌜y ≼ x⌝.
   Proof.
@@ -228,76 +227,10 @@ Section Link_Template.
     { rewrite /(⋅) /=. destruct y; try done. }
     rewrite Hy in Hb. rewrite <- Ha in Hb. done.
   Qed.
-  
-  Lemma auth_ks_included (a1 a2 b1 b2: gset key) : 
-             ✓ prod (a1, b1) → ✓ prod (a2, b2) → prod (a1, b1) ≼ prod (a2, b2) 
-                → (a1 = a2 ∧ b1 = b2) ∨ 
-                    (∃ a0 b0, a2 = a1 ∪ a0 ∧ b2 = b1 ∪ b0 ∧ a1 ## a0 ∧ b1 ## b0 ∧ b1 ⊆ a1 ∧ b2 ⊆ a2 ∧ b0 ⊆ a0).
-  Proof.
-    intros H1 H2 H. destruct H as [z H]. assert (✓ z). { apply (cmra_valid_op_r (prod (a1, b1))).
-    rewrite <-H. done. } rewrite /(✓ prod (a1, b1)) /= in H1. rewrite /(✓ prod (a2, b2)) /= in H2.
-    destruct z.
-    - destruct p. rewrite /(✓ prod (g, g0)) /= in H0. rewrite /(⋅) /= in H.
-      destruct (decide (b1 ⊆ a1)). destruct (decide (g0 ⊆ g)). destruct (decide (a1 ## g)).
-      destruct (decide (b1 ## g0)). right. exists g, g0. set_solver. inversion H. inversion H.
-      inversion H. inversion H.
-    - rewrite /(✓ prodTop) /= in H0. exfalso. done.
-    - rewrite /(⋅) /= in H. inversion H. left. done.
-  Qed.  
-  
-  Lemma auth_ks_local_update_insert K1 C Cn k: 
-              ✓ prod (KS, C) ∧ ✓ prod (K1, Cn) ∧ k ∈ K1 ∧ k ∉ Cn →
-             (prod (KS, C), prod (K1, Cn)) ~l~> (prod (KS, C ∪ {[k]}), prod (K1, Cn ∪ {[k]})).
-  Proof.
-    intros [H1 [H2 [H3 H4]]]. apply local_update_discrete. intros z.
-    intros _. intros. split. rewrite /(✓ prod (KS, C ∪ {[k]})) /=. 
-    rewrite /(cmra_valid keysetRA) /=. rewrite /(✓ prod (KS, C)) /= in H1.
-    assert (k ∈ KS). { apply KS_full. } set_solver. rewrite /(opM) /= in H.
-    destruct z. rewrite /(opM) /=. destruct c. destruct p. rewrite /(op) /= in H.
-    rewrite /(cmra_op keysetRA) /= in H. destruct (decide (Cn ⊆ K1)).
-    destruct (decide (g0 ⊆ g)). destruct (decide (K1 ## g)). destruct (decide (Cn ## g0)).
-    inversion H. rewrite /(op) /=. rewrite /(cmra_op keysetRA) /=. destruct (decide (Cn ∪ {[k]} ⊆ K1)).
-    destruct (decide (g0 ⊆ g)). destruct (decide (K1 ## g)). destruct (decide (Cn ∪ {[k]} ## g0)).
-    assert (Cn ∪ g0 ∪ {[k]} = Cn ∪ {[k]} ∪ g0). { set_solver. } rewrite H0. done.
-    unfold not in n. exfalso. apply n. set_solver. unfold not in n. exfalso. apply n. set_solver.
-    unfold not in n. exfalso. apply n. set_solver. unfold not in n. exfalso. apply n. set_solver.
-    unfold not in n. exfalso. apply n. set_solver. unfold not in n. exfalso. apply n. set_solver.
-    unfold not in n. exfalso. apply n. set_solver. unfold not in n. exfalso. apply n. set_solver.
-    rewrite /(op) /= in H. rewrite /(cmra_op keysetRA) /= in H. inversion H.
-    rewrite /(op) /= in H. rewrite /(cmra_op keysetRA) /= in H. inversion H.
-    rewrite /(op) /=. rewrite /(cmra_op keysetRA) /=. done.
-    rewrite /(opM) /=. inversion H. done.
-  Qed.
-
-  Lemma auth_ks_local_update_delete K1 C Cn k:
-              ✓ prod (KS, C) ∧ ✓ prod (K1, Cn) ∧ k ∈ K1 ∧ k ∈ Cn →
-             (prod (KS, C), prod (K1, Cn)) ~l~> (prod (KS, C ∖ {[k]}), prod (K1, Cn ∖ {[k]})).
-  Proof.
-    intros [H1 [H2 [H3 H4]]]. apply local_update_discrete. intros z.
-    intros _. intros. split. rewrite /(✓ prod (KS, C ∖ {[k]})) /=. 
-    rewrite /(cmra_valid keysetRA) /=. rewrite /(✓ prod (KS, C)) /= in H1.
-    set_solver. rewrite /(opM) /= in H.
-    destruct z. rewrite /(opM) /=. destruct c. destruct p. rewrite /(op) /= in H.
-    rewrite /(cmra_op keysetRA) /= in H. destruct (decide (Cn ⊆ K1)).
-    destruct (decide (g0 ⊆ g)). destruct (decide (K1 ## g)). destruct (decide (Cn ## g0)).
-    inversion H. rewrite /(op) /=. rewrite /(cmra_op keysetRA) /=. destruct (decide (Cn ∖ {[k]} ⊆ K1)).
-    destruct (decide (g0 ⊆ g)). destruct (decide (K1 ## g)). destruct (decide (Cn ∖ {[k]} ## g0)).
-    assert (k ∉ g0). { set_solver. }
-    assert ((Cn ∪ g0) ∖ {[k]} = Cn ∖ {[k]} ∪ g0). { set_solver. } rewrite H7. done.
-    unfold not in n. exfalso. apply n. set_solver. unfold not in n. exfalso. apply n. set_solver.
-    unfold not in n. exfalso. apply n. set_solver. unfold not in n. exfalso. apply n. set_solver.
-    unfold not in n. exfalso. apply n. set_solver. unfold not in n. exfalso. apply n. set_solver.
-    unfold not in n. exfalso. apply n. set_solver. unfold not in n. exfalso. apply n. set_solver.
-    rewrite /(op) /= in H. rewrite /(cmra_op keysetRA) /= in H. inversion H.
-    rewrite /(op) /= in H. rewrite /(cmra_op keysetRA) /= in H. inversion H.
-    rewrite /(op) /=. rewrite /(cmra_op keysetRA) /=. done.
-    rewrite /(opM) /=. inversion H. done.
-  Qed.
-
 
   (* ---------- Lock module proofs ---------- *)
 
-  Lemma lockNode_spec (n: node):
+  Lemma lockNode_spec (n: Node):
     <<< ∀ (b: bool), (lockLoc n) ↦ #b >>>
         lockNode #n    @ ⊤
     <<< (lockLoc n) ↦ #true ∗ if b then False else True, RET #() >>>. (* rewrite if then else *)
@@ -319,7 +252,7 @@ Section Link_Template.
       iModIntro. wp_pures. done.
   Qed.
 
-  Lemma unlockNode_spec (n: node) :
+  Lemma unlockNode_spec (n: Node) :
           <<< lockLoc n ↦ #true >>>
                 unlockNode #n    @ ⊤
           <<< lockLoc n ↦ #false, RET #() >>>.
@@ -339,15 +272,15 @@ Section Link_Template.
 
   Lemma ghost_update_keyset γ_k dop k Cn Cn' res K1 C:
           Ψ dop k Cn Cn' res ∗ own γ_k (● prod (KS, C)) ∗ own γ_k (◯ prod (K1, Cn))
-                             ∗ ⌜Cn' ⊆ K1⌝ ∗ ⌜k ∈ K1⌝  ==∗
+                             ∗ ⌜Cn' ⊆ K1⌝ ∗ ⌜k ∈ K1⌝ ∗ ⌜k ∈ KS⌝  ==∗
                  ∃ C', Ψ dop k C C' res ∗ own γ_k (● prod (KS, C')) ∗ own γ_k (◯ prod (K1, Cn')).
   Proof.
-    iIntros "(#HΨ & Ha & Hf & % & %)". iPoseProof (auth_own_incl_ks γ_k (prod (KS, C)) (prod (K1, Cn))
-                with "[$Ha $Hf]") as "%".
+    iIntros "(#HΨ & Ha & Hf & % & % & HKS)". iPoseProof (auth_own_incl_ks γ_k (prod (KS, C)) (prod (K1, Cn))
+                with "[$Ha $Hf]") as "%". iDestruct "HKS" as %HKS.
     iPoseProof ((own_valid γ_k (● prod (KS, C))) with "Ha") as "%".
     iPoseProof ((own_valid γ_k (◯ prod (K1, Cn))) with "Hf") as "%".
     assert ((K1 = KS ∧ Cn = C) ∨ 
-                    (∃ a0 b0, KS = K1 ∪ a0 ∧ C = Cn ∪ b0 ∧ K1 ## a0 ∧ Cn ## b0 ∧ Cn ⊆ K1 ∧ C ⊆ KS ∧ b0 ⊆ a0)) as Hs.
+            (∃ a0 b0, KS = K1 ∪ a0 ∧ C = Cn ∪ b0 ∧ K1 ## a0 ∧ Cn ## b0 ∧ Cn ⊆ K1 ∧ C ⊆ KS ∧ b0 ⊆ a0)) as Hs.
     { apply (auth_ks_included K1 KS Cn C); try done. apply auth_auth_valid. done. }
     destruct Hs.
     - iEval (unfold Ψ) in "HΨ". destruct H4. destruct dop. 
@@ -357,7 +290,8 @@ Section Link_Template.
       + iDestruct "HΨ" as "%". destruct H6. destruct res.
         * iMod (own_update_2 γ_k (● prod (KS, C)) (◯ prod (K1, Cn)) 
           (● prod (KS, C ∪ {[k]}) ⋅ ◯ prod (K1, Cn ∪ {[k]})) with "[Ha] [Hf]") as "(Ha & Hf)"; try done.
-          { apply auth_update. apply auth_ks_local_update_insert. split; try done. apply auth_auth_valid. done. }
+          { apply auth_update. apply auth_ks_local_update_insert.
+            split; try done. apply auth_auth_valid. done.   }
           iModIntro. iExists (C ∪ {[k]}). iEval (rewrite H6). iFrame.
           unfold Ψ. iPureIntro. split; try done. rewrite <-H5. done.
         * assert (Cn' = Cn). { set_solver. } iModIntro. iExists C. iEval (rewrite <-H8) in "Hf".
@@ -392,18 +326,17 @@ Section Link_Template.
           iFrame. unfold Ψ. iPureIntro. set_solver.
   Qed.
 
-
   (* ---------- Proofs of traverse and searchStrOp ---------- *)
 
-  Lemma traverse_spec (γ γ_fp γ_k: gname) γ_inr γ_fi (k: key) (n: node) (Ns: gset node) (I_n:flowintUR) :
-       ⌜n ∈ Ns⌝ ∗ own γ_fp (◯ Ns) ∗ ⌜root ∈ Ns⌝ ∗ own (γ_inr n) (◯ (inreach I_n n)) ∗ ⌜k ∈ inreach I_n n⌝ -∗ 
-          <<< ∀ C, is_searchStr γ γ_fp γ_k γ_inr γ_fi C >>>
+  Lemma traverse_spec (γ γ_fp γ_k: gname) γ_inr γ_fi root (k: key) (n: Node) (Ns: gset Node) (I_n:flowintUR) :
+       ⌜n ∈ Ns⌝ ∗ own γ_fp (◯ Ns) ∗ ⌜root ∈ Ns⌝ ∗ own (γ_inr n) (◯ (linkset I_n n)) ∗ ⌜k ∈ linkset I_n n⌝ -∗ 
+          <<< ∀ C, is_searchStr γ γ_fp γ_k γ_inr γ_fi root C >>>
                 traverse #n #k
                     @ ⊤
-          <<< ∃ (n': node) (Ns': gsetUR node) (I_n': flowintUR) (Cn': gset key),
-                           is_searchStr γ γ_fp γ_k γ_inr γ_fi C ∗ ⌜n' ∈ Ns'⌝ ∗ own γ_fp (◯ Ns') ∗  hrep n' I_n' Cn' 
-                         ∗ own (γ_fi n') ((●{1/2} I_n')) ∗ own γ_k (◯ prod (ks(n'), Cn')) ∗ ⌜dom I_n' = {[n']}⌝
-                         ∗ ⌜in_inset k I_n' n'⌝ ∗ ⌜not_in_outset k I_n'⌝, RET #n' >>>.
+          <<< ∃ (n': Node) (Ns': gsetUR Node) (I_n': flowintUR) (Cn': gset key),
+                           is_searchStr γ γ_fp γ_k γ_inr γ_fi root C ∗ ⌜n' ∈ Ns'⌝ ∗ own γ_fp (◯ Ns') ∗ node n' I_n' Cn' 
+                         ∗ own (γ_fi n') ((●{1/2} I_n')) ∗ own γ_k (◯ prod (keyset I_n' n', Cn')) ∗ ⌜dom I_n' = {[n']}⌝
+                         ∗ ⌜in_inset k I_n' n'⌝ ∗ ⌜¬in_outsets k I_n'⌝, RET #n' >>>.
   Proof.
     iLöb as "IH" forall (n Ns I_n). iIntros "(#Hinn & #Hfp & #Hroot & #Hinrfp & #Hkinr)".
     iDestruct "Hinn" as %Hinn. iDestruct "Hroot" as %Hroot.
@@ -421,14 +354,14 @@ Section Link_Template.
     iFrame "# % ∗". eauto with iFrame. } iIntros "(Hloc & ?)".
     destruct b. { iExFalso. done. } iModIntro. 
     iPoseProof (auth_set_incl with "[$Hks $Hinrfp]") as "%".
-    iDestruct "Hkinr" as "%". assert (k ∈ inreach In n) as Hkinr. { set_solver. }
+    iDestruct "Hkinr" as "%". assert (k ∈ linkset In n) as Hkinr. { set_solver. }
     iPoseProof (own_valid with "HIn") as "%". rename H2 into HInV.
     assert (✓ In) as HInv. { apply (auth_frag_valid (◯ In)). done. }
     iSplitR "Hb". iFrame "∗ % #". iExists I. iFrame "∗ % #". iApply "Hstar". iExists true, In.
     iFrame "# % ∗". iIntros "AU". iModIntro. wp_pures.
     iDestruct "Hb" as (Cn) "(Hrep & Hfil & Hks)". iDestruct "HNds" as %HNds.
     wp_bind (findNext _ _)%E. wp_apply ((findNext_spec n In Cn k) with "[Hrep]").
-    iFrame; iPureIntro; done. iIntros (b n') "(Hrep & Hb)". destruct b. 
+    iFrame; iPureIntro; left; done. iIntros (b n') "(Hrep & Hb)". destruct b. 
     - wp_pures. awp_apply (unlockNode_spec n). 
       iApply (aacc_aupd_abort with "AU"); first done. iIntros (C1) "Hst".
       iDestruct "Hst" as (I1) "(HI & HKS & HNDS & Hglob & Hstar)".
@@ -438,14 +371,14 @@ Section Link_Template.
       rewrite (big_sepS_delete _ (dom I1) n); last by eauto. iDestruct "Hstar" as "(Hcln & Hstar)".
       iDestruct "Hcln" as (b In1) "(Hlock & Hbb & HIn & #HNds1 & Hfis & Hks1)".
       destruct b; first last. { iDestruct "Hbb" as (Cn') "(Hrep' & _)".
-      iAssert (⌜False⌝)%I with "[Hrep Hrep']" as %Hf. { iApply (hrep_sep_star n In In1). 
+      iAssert (⌜False⌝)%I with "[Hrep Hrep']" as %Hf. { iApply (node_sep_star n In In1). 
       iFrame. } exfalso. done. }
       iPoseProof ((own_valid_2 (γ_fi n) (●{1 / 2} In) (●{1 / 2} In1)) with "[Hfil] [Hfis]") as "%"; try done.
       apply (auth_auth_frac_op_inv _ _ _ _) in H3. apply leibniz_equiv in H3. replace In1.            
       iDestruct "Hb" as %Hb. iDestruct "HNds1" as %HNds1. iDestruct "Hglob" as %Hglob.
       iPoseProof (auth_own_incl with "[$HI $HIn]") as (I2)"%".
       iPoseProof (own_valid with "HI") as "%". iAssert (⌜n' ∈ dom I1⌝)%I as "%".
-      { iPureIntro. assert (n' ∈ dom I2). { apply (flowint_step I1 In I2 k n'). done. 
+      { iPureIntro. assert (n' ∈ dom I2). { apply (flowint_step I1 In I2 k n' root). done. 
         apply auth_auth_valid. done. done. done. }
         apply flowint_comp_fp in H4. set_solver. }
       assert (n ≠ n') as Hneq. { assert (n' ∉ dom In). { apply (outset_distinct In n').
@@ -456,10 +389,10 @@ Section Link_Template.
       iPoseProof ((own_op γ (◯ In) (◯ In' )) with "[HIn HIn']") as "H"; first by eauto with iFrame.
       iPoseProof (own_valid with "H") as "%". rewrite -auth_frag_op in H7.
       assert (✓ (In ⋅ In')). { apply (auth_frag_valid (◯ (In ⋅ In'))). done. }
-      iDestruct "HNds'" as %HNds'. assert (k ∈ inreach In' n').
-      { apply (flowint_inreach_step (In⋅In') In In' k n n'); try done. set_solver. }
+      iDestruct "HNds'" as %HNds'. assert (k ∈ linkset In' n').
+      { apply (flowint_inreach_step (In⋅In') In In' k n n'); try done. }
       assert (root ∈ dom I1). { apply globalint_root_fp. done. } iDestruct "H" as "(HIn & HIn')".
-      iMod (own_update (γ_inr n') (● inreach In' n') (● inreach In' n' ⋅ ◯ inreach In' n') with "Hks1'") as "HNs".
+      iMod (own_update (γ_inr n') (● linkset In' n') (● linkset In' n' ⋅ ◯ linkset In' n') with "Hks1'") as "HNs".
       apply auth_update_core_id. apply gset_core_id. done. iDestruct "HNs" as "(Hks1' & #Hinr1')".
       iAaccIntro with "Hlock". { iIntros "Hlock". iModIntro. iSplitR "Hfil Hks Hrep". iFrame "∗ # %".
       iExists I1. iFrame "∗ % #". rewrite (big_sepS_delete _ (dom I1) n); last by eauto.
@@ -475,23 +408,23 @@ Section Link_Template.
       iApply "IH". iFrame "∗ # %". done.
     - iApply fupd_wp. iMod "AU" as (C) "[Hst [_ Hclose]]". iSpecialize ("Hclose" $! n Ns In Cn).
       iMod ("Hclose" with "[Hst Hfil Hks Hrep Hb]") as "HΦ". iDestruct "Hb" as %Hnotout.
-      iFrame "∗ # %". iPureIntro. apply (inreach_impl_inset In n k); try split; try done.
-      iModIntro. wp_pures. done.
+      iAssert (node n In Cn ∗ ⌜nodeinv In n⌝)%I with "[Hrep]" as "(Hrep & Hninv)". 
+      { iApply (node_implies_nodeinv _ _ _). iFrame "∗ # %". } iDestruct "Hninv" as %Hninv. 
+      iFrame "∗ # %". iPureIntro. unfold nodeinv in Hninv. specialize (Hninv k).
+      apply Hninv. try done. iModIntro. wp_pures. done.
   Qed.
 
-
-
-  Theorem searchStrOp_spec (γ γ_fp γ_k: gname) γ_inr γ_fi (k: key) (dop: dOp):
-      <<< ∀ C, is_searchStr γ γ_fp γ_k γ_inr γ_fi C >>>
+  Theorem searchStrOp_spec (γ γ_fp γ_k: gname) γ_inr γ_fi root (k: key) (dop: dOp):
+      ⌜k ∈ KS⌝ -∗ <<< ∀ C, is_searchStr γ γ_fp γ_k γ_inr γ_fi root C >>>
             searchStrOp dop root #k
                   @ ⊤
-      <<< ∃ C' (res: bool), is_searchStr γ γ_fp γ_k γ_inr γ_fi C' 
+      <<< ∃ C' (res: bool), is_searchStr γ γ_fp γ_k γ_inr γ_fi root C' 
                                         ∗ Ψ dop k C C' res, RET #res >>>.
   Proof.
-    iIntros (Φ) "AU". iLöb as "IH". wp_lam.
+    iIntros "HKin" (Φ) "AU". iLöb as "IH". wp_lam.
     iApply fupd_wp. iMod "AU" as (C0) "[Hst [HAU _]]".
     iDestruct "Hst" as (I0) "(HI & HKS & HNDS & #Hglob & Hstar)".
-    iDestruct "Hglob" as %Hglob. 
+    iDestruct "Hglob" as %Hglob. iDestruct "HKin" as %HKin. 
     assert (root ∈ dom I0)%I as Hroot. { apply globalint_root_fp. done. }
     iMod (own_update γ_fp (● dom I0) (● dom I0 ⋅ ◯ dom I0) with "HNDS") as "H".
     { apply auth_update_core_id. apply gset_core_id. done. } 
@@ -500,14 +433,14 @@ Section Link_Template.
     iDestruct "Hstar" as "[Hn Hstar]".
     iDestruct "Hn" as (b Ir) "(H1 & H2 & H3 & H4 & H5 & Hksr)".
     iPoseProof (auth_own_incl with "[$HI $H3]") as "%". iDestruct "H4" as %HNdsr.
-    assert (inreach Ir root = inreach I0 root) as Hinreach. { apply globalint_inreach; try done. }
-    iMod (own_update (γ_inr root) (● inreach Ir root) (● inreach Ir root ⋅ ◯ inreach Ir root) with "Hksr") as "H".
+    (*assert (inreach Ir root = inreach I0 root) as Hinreach. { apply globalint_inreach; try done. }*)
+    iMod (own_update (γ_inr root) (● linkset Ir root) (● linkset Ir root ⋅ ◯ linkset Ir root) with "Hksr") as "H".
     apply auth_update_core_id. apply gset_core_id. done. iDestruct "H" as "(Hksr & #Hinr)".
     iMod ("HAU" with "[HI HKS H1 H2 H3 H5 Hstar HNDS Hksr] ") as "AU". 
     { iExists I0. iFrame "∗ % #". iApply "Hstar". iExists b, Ir. iFrame "∗ # %". }
     iModIntro. wp_bind (traverse _ _)%E.
-    awp_apply (traverse_spec γ γ_fp γ_k γ_inr γ_fi k root (dom I0) Ir). iFrame "∗ # %".
-    iPureIntro. rewrite Hinreach. apply globalint_root_inr. done.
+    awp_apply (traverse_spec γ γ_fp γ_k γ_inr γ_fi root k root (dom I0) Ir). iFrame "∗ # %".
+    iPureIntro. apply (globalint_root_inr I0 Ir root k); try done.
     iApply (aacc_aupd_abort with "AU"); first done.
     iIntros (C1) "Hst". iAaccIntro with "Hst"; first by eauto with iFrame.
     iIntros (n Ns In Cn) "(Hst & #Hinn & #Hfp & Hrepn & Hfil & Hks & #HNdsn & #Hinset & #Hnotout)".
@@ -528,7 +461,7 @@ Section Link_Template.
       iDestruct "Hstar" as "[Hn Hstar]".
       iDestruct "Hn" as (b' In1) "(Hlock & Hb & HIn & #HNds & Hfis & Hinreach)".
       destruct b'; first last. { iDestruct "Hb" as (Cn'') "(Hrep' & _)".
-      iAssert (⌜False⌝)%I with "[Hrep Hrep']" as %Hf. { iApply (hrep_sep_star n In In1). 
+      iAssert (⌜False⌝)%I with "[Hrep Hrep']" as %Hf. { iApply (node_sep_star n In In1). 
       iFrame. } exfalso. done. }
       iAaccIntro with "Hlock". { iIntros "Hlock". iModIntro. iSplitR "Hfil Hrep Hks".
       iExists I. iFrame "∗ % #". iApply "Hstar". iExists true, In1. 
@@ -536,9 +469,13 @@ Section Link_Template.
       iPoseProof (auth_own_incl with "[$HI $HIn]") as (I2)"%".
       iPoseProof ((own_valid γ (● I)) with "HI") as "%".
       iPoseProof ((own_valid_2 (γ_fi n) (●{1 / 2} In) (●{1 / 2} In1)) with "[Hfil] [Hfis]") as "%"; try done.
-      apply (auth_auth_frac_op_inv _ _ _ _) in H3. apply leibniz_equiv in H3. replace In1.            
-      iMod ((ghost_update_keyset γ_k dop k Cn Cn' res (ks n) C2) with "[HKS Hks]") as "Hgks".
-      iFrame "% ∗ #". iPureIntro. apply (keyset_in_out k In n); try done. 
+      apply (auth_auth_frac_op_inv _ _ _ _) in H3. apply leibniz_equiv in H3. replace In1.
+      iPoseProof ((own_valid γ (◯ In)) with "HIn") as "%". rename H4 into HInV.
+      assert (✓ In) as HInv. { apply (auth_frag_valid (◯ In)). done. }
+      iAssert (node n In Cn' ∗ ⌜nodeinv In n⌝)%I with "[Hrep]" as "(Hrep & Hninv)". 
+      { iApply (node_implies_nodeinv _ _ _). iFrame "% ∗ #". } iDestruct "Hninv" as %Hninv.                   
+      iMod ((ghost_update_keyset γ_k dop k Cn Cn' res (keyset In n) C2) with "[HKS Hks]") as "Hgks".
+      iFrame "% ∗ #". iPureIntro. apply keyset_def; try done.
       iDestruct "Hgks" as (C2') "(#HΨC & Ha & Hf)".
       iModIntro. iExists (C2'), res. iSplitL. iSplitR "HΨC".
       { iExists I. iFrame "∗ % #".
@@ -556,7 +493,7 @@ Section Link_Template.
       iDestruct "Hstar" as "[Hn Hstar]".
       iDestruct "Hn" as (b' In1) "(Hlock & Hb' & HIn & #HNds & Hfis & Hinreach)".
       destruct b'; first last. { iDestruct "Hb'" as (Cn'') "(Hrep' & _)".
-      iAssert (⌜False⌝)%I with "[Hb Hrep']" as %Hf. { iApply (hrep_sep_star n In In1). 
+      iAssert (⌜False⌝)%I with "[Hb Hrep']" as %Hf. { iApply (node_sep_star n In In1). 
       iFrame "∗ # %". } exfalso. done. }
       iAaccIntro with "Hlock". { iIntros "Hlock". iModIntro. iSplitR "Hfil Hb Hks".
       iExists I. iFrame "∗ % #". iApply "Hstar". iExists true, In1. 
@@ -564,23 +501,7 @@ Section Link_Template.
       iPoseProof ((own_valid_2 (γ_fi n) (●{1 / 2} In) (●{1 / 2} In1)) with "[Hfil] [Hfis]") as "%"; try done.
       apply (auth_auth_frac_op_inv _ _ _ _) in H1. apply leibniz_equiv in H1. replace In1.            
       iSplitR "". iExists I. iFrame "∗ % #". iApply "Hstar". iExists false, In. iFrame "∗ % #".
-      iExists Cn. iFrame. iIntros "AU". iModIntro. wp_pures. iApply "IH". done.
+      iExists Cn. iFrame. iIntros "AU". iModIntro. wp_pures. iApply "IH"; try done.
   Qed.
  
-
-
-
-
-
-
-
-
-
-
-
-
-
-
-
-
 
